Documentation, renaming and reorganization of the memory model

src/coq/Handlers/Memory.v
@@ -8,7 +8,7 @@
  *   3 of the License, or (at your option) any later version.                 *
  ---------------------------------------------------------------------------- *)
 
-
+(* begin hide *)
 From Coq Require Import
      Morphisms ZArith List String Omega
      FSets.FMapAVL
@@ -50,7 +50,20 @@ Import ListNotations.
 
 Set Implicit Arguments.
 Set Contextual Implicit.
+(* end hide *)
 
+(** * Memory Model
+
+    This file implements VIR's memory model as an handler for the [MemoryE] family of events.
+    The model is inspired by CompCert's memory model, but differs in that it maintains two
+    representation of the memory, a logical one and a low-level one.
+    Pointers (type signature [MemoryAddress.ADDRESS]) are implemented as a pair containing
+    an address and an offset. 
+*)
+
+(** ** Type of pointers
+    Implementation of the notion of pointer used: an address and an offset.
+ *)
 Module Addr : MemoryAddress.ADDRESS with Definition addr := (Z * Z) % type.
   Definition addr := (Z * Z) % type.
   Definition null := (0, 0).
@@ -67,6 +80,11 @@ Module Addr : MemoryAddress.ADDRESS with Definition addr := (Z * Z) % type.
   Qed.
 End Addr.
 
+(** ** Memory model
+    Implementation of the memory model, i.e. a handler for [MemoryE].
+    The memory itself, [memory], is a finite map (using the standard library's AVLs)
+    indexed on [Z].
+ *)
 Module Make(LLVMEvents: LLVM_INTERACTIONS(Addr)).
   Import LLVMEvents.
   Import DV.
@@ -75,6 +93,7 @@ Module Make(LLVMEvents: LLVM_INTERACTIONS(Addr)).
   Definition addr := Addr.addr.
 
   Module IM := FMapAVL.Make(Coq.Structures.OrderedTypeEx.Z_as_OT).
+  (* Polymorphic type of maps indexed by [Z] *)
   Definition IntMap := IM.t.
 
   Definition add {a} k (v:a) := IM.add k v.
@@ -83,20 +102,26 @@ Module Make(LLVMEvents: LLVM_INTERACTIONS(Addr)).
   Definition lookup {a} k (m:IntMap a) := IM.find k m.
   Definition empty {a} := @IM.empty a.
 
+  (* Extends the map with a list of pairs key/value.
+     Note: additions start from the end of the list, so in case of duplicate
+     keys, the binding in the front will shadow though in the back.
+   *)
   Fixpoint add_all {a} ks (m:IntMap a) :=
     match ks with
     | [] => m
     | (k,v) :: tl => add k v (add_all tl m)
     end.
 
+  (* Extends the map with the bindings {(i,v_1) .. (i+n-1, v_n)} for [vs ::= v_1..v_n] *)
   Fixpoint add_all_index {a} vs (i:Z) (m:IntMap a) :=
     match vs with
     | [] => m
     | v :: tl => add i v (add_all_index tl (i+1) m)
     end.
 
-  (* Give back a list of values from i to (i + sz) - 1 in m. *)
-  (* Uses def as the default value if a lookup failed. *)
+  (* Give back a list of values from [|i|] to [|i| + |sz| - 1] in [m].
+     Uses [def] as the default value if a lookup failed.
+   *)
   Definition lookup_all_index {a} (i:Z) (sz:Z) (m:IntMap a) (def:a) : list a :=
     List.map (fun x =>
                 let x' := lookup (Z.of_nat x) m in
@@ -105,23 +130,27 @@ Module Make(LLVMEvents: LLVM_INTERACTIONS(Addr)).
                 | Some val => val
                 end) (seq (Z.to_nat i) (Z.to_nat sz)).
 
+  (* Takes the join of two maps, favoring the first one over the intersection of their domains *)
   Definition union {a} (m1 : IntMap a) (m2 : IntMap a)
     := IM.map2 (fun mx my =>
                   match mx with | Some x => Some x | None => my end) m1 m2.
 
+  (* TODO : Move the three following functions *)
+    Fixpoint max_default (l:list Z) (x:Z) :=
+    match l with
+    | [] => x
+    | h :: tl =>
+      max_default tl (if h >? x then h else x)
+    end.
+
   Definition maximumBy {A} (leq : A -> A -> bool) (def : A) (l : list A) : A :=
     fold_left (fun a b => if leq a b then b else a) l def.
 
-  (* Get a fresh key for use in memory map *)
-  Definition next_key {a} (m : IM.t a) : Z
-    := let keys := map fst (IM.elements m) in
-       1 + maximumBy Z.leb (-1) keys.
-
-  Inductive SByte :=
-  | Byte : byte -> SByte
-  | Ptr : addr -> SByte
-  | PtrFrag : SByte
-  | SUndef : SByte.
+  Definition is_some {A} (o : option A) :=
+    match o with
+    | Some x => true
+    | None => false
+    end.
 
   (* TODO SAZ: mem_block should keep track of its allocation size so
     that operations can fail if they are out of range
@@ -131,211 +160,253 @@ Module Make(LLVMEvents: LLVM_INTERACTIONS(Addr)).
     lookup functions handle this properly, anyway.
    *)
 
-  (* Simple view of memory *)
-  Inductive concrete_block :=
-  | CBlock (size : Z) (block_id : Z) : concrete_block.
+  Section Datatype_Definition.
 
-  Inductive logical_block :=
-  | LBlock (size : Z) (bytes : IntMap SByte) (concrete_id : option Z) : logical_block.
+    (** ** Simple view of memory
+      A concrete block is determined by its id and its size.
+     *)
+    Inductive concrete_block :=
+    | CBlock (size : Z) (block_id : Z) : concrete_block.
 
-  Definition mem_block       := IntMap SByte.
+    (** ** Logical view of memory
+      A logical block is determined by a size and a mapping from [Z] to special bytes,
+      we call such a mapping a [mem_block].
+      Those bytes can either be an actually 8bits byte, an address of a pointer,
+      a [PtrFrag], marking bytes that are part of an address but not its first byte,
+      or a special undefined byte.
+      It may also correspond to a concrete block whose id is then provided.
+     *)
+    Inductive SByte :=
+    | Byte : byte -> SByte
+    | Ptr : addr -> SByte
+    | PtrFrag : SByte
+    | SUndef : SByte.
+    Definition mem_block       := IntMap SByte.
+    Inductive logical_block :=
+    | LBlock (size : Z) (bytes : mem_block) (concrete_id : option Z) : logical_block.
 
-  Definition concrete_memory := IntMap concrete_block.
-  Definition logical_memory  := IntMap logical_block.
-  Definition memory          := (concrete_memory * logical_memory)%type.
+    (** ** Memory
+      A concrete memory, resp. logical memory, maps addresses to concrete blocks, resp. logical blocks.
+      A memory is a pair of both views of the memory.
+     *)
+    Definition concrete_memory := IntMap concrete_block.
+    Definition logical_memory  := IntMap logical_block.
+    Definition memory          := (concrete_memory * logical_memory)%type.
 
-  (* Stack frames *)
-  Definition mem_frame := list Z.  (* A list of block ids that need to be freed when popped *)
-  Definition mem_stack := list mem_frame.
+    (** ** Stack frames
+      A frame contains the list of block ids that need to be freed when popped,
+      i.e. when the function returns.
+      A [frame_stack] is a list of such frames.
+     *)
+    Definition mem_frame := list Z.  
+    Definition frame_stack := list mem_frame.
 
-  (* Memory + stack for freeing *)
-  Definition memory_stack : Type := memory * mem_stack.
+    (** ** Memory stack
+      The full notion of state manipulated by the monad is a pair of a [memory] and a [mem_stack].
+     *)
+    Definition memory_stack : Type := memory * frame_stack.
 
-  Definition empty_memory_stack : memory_stack := ((empty, empty), [[]]).
+  End Datatype_Definition.
 
-  Fixpoint max_default (l:list Z) (x:Z) :=
-    match l with
-    | [] => x
-    | h :: tl =>
-      max_default tl (if h >? x then h else x)
-    end.
+  Section Serialization.
 
-  (* Computes the byte size of this type. *)
-  Fixpoint sizeof_dtyp (ty:dtyp) : Z :=
-    match ty with
-    | DTYPE_I sz => 8 (* All integers are padded to 8 bytes. *)
-    | DTYPE_Pointer => 8
-    | DTYPE_Struct l => fold_left (fun x acc => x + sizeof_dtyp acc) l 0
-    | DTYPE_Array sz ty' => sz * sizeof_dtyp ty'
-    | DTYPE_Float => 4
-    | DTYPE_Double => 8
-    | _ => 0 (* TODO: add support for more types as necessary *)
-    end.
+   (** ** Serialization
+       Conversion back and forth between values and their byte representation
+   *) 
 
-  (* Convert integer to its byte representation. *)
-  Fixpoint bytes_of_int (n: nat) (x: Z) {struct n}: list byte :=
-    match n with
-    | O => nil
-    | S m => Byte.repr x :: bytes_of_int m (x / 256)
-    end.
+    (* Converts an integer [x] to its byte representation over [n] bytes.
+     The representation is little endian. In particular, if [n] is too small,
+     only the least significant bytes are returned.
+     *)
+    Fixpoint bytes_of_int (n: nat) (x: Z) {struct n}: list byte :=
+      match n with
+      | O => nil
+      | S m => Byte.repr x :: bytes_of_int m (x / 256)
+      end.
 
-  Fixpoint int_of_bytes (l: list byte): Z :=
-    match l with
-    | nil => 0
-    | b :: l' => Byte.unsigned b + int_of_bytes l' * 256
-    end.
+    Definition sbytes_of_int (count:nat) (z:Z) : list SByte :=
+      List.map Byte (bytes_of_int count z).
 
-  (* CB TODO: Is interpreting everything except for bytes as undef reasonable? *)
-  Definition Sbyte_to_byte (sb:SByte) : option byte :=
-    match sb with
-    | Byte b => ret b
-    | Ptr _ | PtrFrag | SUndef => None
-    end.
+    (* Converts a list of bytes to an integer.
+     The byte encoding is assumed to be little endian.
+     *)
+    Fixpoint int_of_bytes (l: list byte): Z :=
+      match l with
+      | nil => 0
+      | b :: l' => Byte.unsigned b + int_of_bytes l' * 256
+      end.
 
-  Definition Z_to_sbyte_list (count:nat) (z:Z) : list SByte :=
-    List.map Byte (bytes_of_int count z).
+    (* Partial function casting a [Sbyte] into a simple [byte] *)
+    (* CB TODO: Is interpreting everything except for bytes as undef reasonable? *)
+    Definition Sbyte_to_byte (sb:SByte) : option byte :=
+      match sb with
+      | Byte b => ret b
+      | Ptr _ | PtrFrag | SUndef => None
+      end.
 
-  Definition Sbyte_to_byte_list (sb:SByte) : list byte :=
-    match sb with
-    | Byte b => [b]
-    | Ptr _ | PtrFrag | SUndef => []
-    end.
+    Definition Sbyte_to_byte_list (sb:SByte) : list byte :=
+      match sb with
+      | Byte b => [b]
+      | Ptr _ | PtrFrag | SUndef => []
+      end.
 
-  Definition sbyte_list_to_byte_list (bytes:list SByte) : list byte :=
-    List.flat_map Sbyte_to_byte_list bytes.
+    Definition sbyte_list_to_byte_list (bytes:list SByte) : list byte :=
+      List.flat_map Sbyte_to_byte_list bytes.
 
-  Definition sbyte_list_to_Z (bytes:list SByte) : Z :=
-    int_of_bytes (sbyte_list_to_byte_list bytes).
+    Definition sbyte_list_to_Z (bytes:list SByte) : Z :=
+      int_of_bytes (sbyte_list_to_byte_list bytes).
 
+    (** Length properties *)
 
-  (** Length properties *)
+    Lemma length_bytes_of_int:
+      forall n x, List.length (bytes_of_int n x) = n.
+    Proof.
+      induction n; simpl; intros. auto. decEq. auto.
+    Qed.
 
-  Lemma length_bytes_of_int:
-    forall n x, List.length (bytes_of_int n x) = n.
-  Proof.
-    induction n; simpl; intros. auto. decEq. auto.
-  Qed.
+    Lemma int_of_bytes_of_int:
+      forall n x,
+        int_of_bytes (bytes_of_int n x) = x mod (two_p (Z.of_nat n * 8)).
+    Proof.
+      induction n; intros.
+      simpl. rewrite Zmod_1_r. auto.
+      Opaque Byte.wordsize.
+      rewrite Nat2Z.inj_succ. simpl.
+      replace (Z.succ (Z.of_nat n) * 8) with (Z.of_nat n * 8 + 8) by omega.
+      rewrite two_p_is_exp; try omega.
+      rewrite Zmod_recombine. rewrite IHn. rewrite Z.add_comm.
+      change (Byte.unsigned (Byte.repr x)) with (Byte.Z_mod_modulus x).
+      rewrite Byte.Z_mod_modulus_eq. reflexivity.
+      apply two_p_gt_ZERO. omega. apply two_p_gt_ZERO. omega.
+    Qed.
 
-  Lemma int_of_bytes_of_int:
-    forall n x,
-      int_of_bytes (bytes_of_int n x) = x mod (two_p (Z.of_nat n * 8)).
-  Proof.
-    induction n; intros.
-    simpl. rewrite Zmod_1_r. auto.
-    Opaque Byte.wordsize.
-    rewrite Nat2Z.inj_succ. simpl.
-    replace (Z.succ (Z.of_nat n) * 8) with (Z.of_nat n * 8 + 8) by omega.
-    rewrite two_p_is_exp; try omega.
-    rewrite Zmod_recombine. rewrite IHn. rewrite Z.add_comm.
-    change (Byte.unsigned (Byte.repr x)) with (Byte.Z_mod_modulus x).
-    rewrite Byte.Z_mod_modulus_eq. reflexivity.
-    apply two_p_gt_ZERO. omega. apply two_p_gt_ZERO. omega.
-  Qed.
+    (** ** Serialization of [dvalue]
+      Serializes a dvalue into its SByte-sensitive form.
+      Integer are stored over 8 bytes.
+      Pointers as well: the address is stored in the first, [PtrFrag] flags mark the seven others.
+     *)
+    Fixpoint serialize_dvalue (dval:dvalue) : list SByte :=
+      match dval with
+      | DVALUE_Addr addr => (Ptr addr) :: (repeat PtrFrag 7)
+      | DVALUE_I1 i => sbytes_of_int 8 (unsigned i)
+      | DVALUE_I8 i => sbytes_of_int 8 (unsigned i)
+      | DVALUE_I32 i => sbytes_of_int 8 (unsigned i)
+      | DVALUE_I64 i => sbytes_of_int 8 (unsigned i)
+      | DVALUE_Float f => sbytes_of_int 4 (unsigned (Float32.to_bits f))
+      | DVALUE_Double d => sbytes_of_int 8 (unsigned (Float.to_bits d))
+      | DVALUE_Struct fields
+      | DVALUE_Array fields =>
+        (* note the _right_ fold is necessary for byte ordering. *)
+        fold_right (fun 'dv acc => ((serialize_dvalue dv) ++ acc) % list) [] fields
+      | _ => [] (* TODO add more dvalues as necessary *)
+      end.
 
-  (* Serializes a dvalue into its SByte-sensitive form. *)
-  Fixpoint serialize_dvalue (dval:dvalue) : list SByte :=
-    match dval with
-    | DVALUE_Addr addr => (Ptr addr) :: (repeat PtrFrag 7)
-    | DVALUE_I1 i => Z_to_sbyte_list 8 (unsigned i)
-    | DVALUE_I8 i => Z_to_sbyte_list 8 (unsigned i)
-    | DVALUE_I32 i => Z_to_sbyte_list 8 (unsigned i)
-    | DVALUE_I64 i => Z_to_sbyte_list 8 (unsigned i)
-    | DVALUE_Float f => Z_to_sbyte_list 4 (unsigned (Float32.to_bits f))
-    | DVALUE_Double d => Z_to_sbyte_list 8 (unsigned (Float.to_bits d))
-    | DVALUE_Struct fields | DVALUE_Array fields =>
-                             (* note the _right_ fold is necessary for byte ordering. *)
-                             fold_right (fun 'dv acc => ((serialize_dvalue dv) ++ acc) % list) [] fields
-    | _ => [] (* TODO add more dvalues as necessary *)
-    end.
+    (** ** Well defined block
+      A list of [sbytes] is considered undefined if any of its bytes is undefined.
+      This predicate checks that they are all well-defined.
+     *)
+    Definition all_not_sundef (bytes : list SByte) : bool :=
+      forallb is_some (map Sbyte_to_byte bytes).
 
-  (* CB TODO: does this really not exist somewhere? *)
-  Definition is_some {A} (o : option A) :=
-    match o with
-    | Some x => true
-    | None => false
-    end.
+    (** ** Size of a dynamic type
+      Computes the byte size of a [dtyp]. *)
+    Fixpoint sizeof_dtyp (ty:dtyp) : Z :=
+      match ty with
+      | DTYPE_I sz         => 8 (* All integers are padded to 8 bytes. *)
+      | DTYPE_Pointer      => 8
+      | DTYPE_Struct l     => fold_left (fun x acc => x + sizeof_dtyp acc) l 0
+      | DTYPE_Array sz ty' => sz * sizeof_dtyp ty'
+      | DTYPE_Float        => 4
+      | DTYPE_Double       => 8
+      | _                  => 0 (* TODO: add support for more types as necessary *)
+      end.
 
-  Definition all_not_sundef (bytes : list SByte) : bool :=
-    forallb is_some (map Sbyte_to_byte bytes).
+    (** ** Deserialization of a list of sbytes
+      Deserialize a list [bytes] of SBytes into a uvalue of type [t],
+      assuming that none of the bytes are undef.
+      Truncate integer as dictated by [t].
+     *)
+    Fixpoint deserialize_sbytes_defined (bytes:list SByte) (t:dtyp) : uvalue :=
+      match t with
+      | DTYPE_I sz =>
+        let des_int := sbyte_list_to_Z bytes in
+        match sz with
+        | 1  => UVALUE_I1 (repr des_int)
+        | 8  => UVALUE_I8 (repr des_int)
+        | 32 => UVALUE_I32 (repr des_int)
+        | 64 => UVALUE_I64 (repr des_int)
+        | _  => UVALUE_None (* invalid size. *)
+        end
+      | DTYPE_Float => UVALUE_Float (Float32.of_bits (repr (sbyte_list_to_Z bytes)))
+      | DTYPE_Double => UVALUE_Double (Float.of_bits (repr (sbyte_list_to_Z bytes)))
 
-  (* Deserialize a list of SBytes into a uvalue, assuming that none of the bytes are undef *)
-  Fixpoint deserialize_sbytes_defined (bytes:list SByte) (t:dtyp) : uvalue :=
-    match t with
-    | DTYPE_I sz =>
-      let des_int := sbyte_list_to_Z bytes in
-      match sz with
-      | 1  => UVALUE_I1 (repr des_int)
-      | 8  => UVALUE_I8 (repr des_int)
-      | 32 => UVALUE_I32 (repr des_int)
-      | 64 => UVALUE_I64 (repr des_int)
-      | _  => UVALUE_None (* invalid size. *)
-      end
-    | DTYPE_Float => UVALUE_Float (Float32.of_bits (repr (sbyte_list_to_Z bytes)))
-    | DTYPE_Double => UVALUE_Double (Float.of_bits (repr (sbyte_list_to_Z bytes)))
+      | DTYPE_Pointer =>
+        match bytes with
+        | Ptr addr :: tl => UVALUE_Addr addr
+        | _ => UVALUE_None (* invalid pointer. *)
+        end
+      | DTYPE_Array sz t' =>
+        let fix array_parse count byte_sz bytes :=
+            match count with
+            | O => []
+            | S n => (deserialize_sbytes_defined (firstn byte_sz bytes) t')
+                      :: array_parse n byte_sz (skipn byte_sz bytes)
+            end in
+        UVALUE_Array (array_parse (Z.to_nat sz) (Z.to_nat (sizeof_dtyp t')) bytes)
+      | DTYPE_Struct fields =>
+        let fix struct_parse typ_list bytes :=
+            match typ_list with
+            | [] => []
+            | t :: tl =>
+              let size_ty := Z.to_nat (sizeof_dtyp t) in
+              (deserialize_sbytes_defined (firstn size_ty bytes) t)
+                :: struct_parse tl (skipn size_ty bytes)
+            end in
+        UVALUE_Struct (struct_parse fields bytes)
+      | _ => UVALUE_None (* TODO add more as serialization support increases *)
+      end.
 
-    | DTYPE_Pointer =>
-      match bytes with
-      | Ptr addr :: tl => UVALUE_Addr addr
-      | _ => UVALUE_None (* invalid pointer. *)
-      end
-    | DTYPE_Array sz t' =>
-      let fix array_parse count byte_sz bytes :=
-          match count with
-          | O => []
-          | S n => (deserialize_sbytes_defined (firstn byte_sz bytes) t')
-                     :: array_parse n byte_sz (skipn byte_sz bytes)
-          end in
-      UVALUE_Array (array_parse (Z.to_nat sz) (Z.to_nat (sizeof_dtyp t')) bytes)
-    | DTYPE_Struct fields =>
-      let fix struct_parse typ_list bytes :=
-          match typ_list with
-          | [] => []
-          | t :: tl =>
-            let size_ty := Z.to_nat (sizeof_dtyp t) in
-            (deserialize_sbytes_defined (firstn size_ty bytes) t)
-              :: struct_parse tl (skipn size_ty bytes)
-          end in
-      UVALUE_Struct (struct_parse fields bytes)
-    | _ => UVALUE_None (* TODO add more as serialization support increases *)
-    end.
+    (* Returns undef if _any_ sbyte is undef.
+     Note that this means for instance that the result of the deserialization of an I1
+     depends on all the bytes provided, not just the first one!
+     *)
+    Definition deserialize_sbytes (bytes : list SByte) (t : dtyp) : uvalue :=
+      if all_not_sundef bytes
+      then deserialize_sbytes_defined bytes t
+      else UVALUE_Undef t.
 
-  Definition deserialize_sbytes (bytes : list SByte) (t : dtyp) : uvalue :=
-    if all_not_sundef bytes
-    then deserialize_sbytes_defined bytes t
-    else UVALUE_Undef t.
+    (* Todo - complete proofs, and think about moving to MemoryProp module. *)
+    (* The relation defining serializable dvalues. *)
+    Inductive serialize_defined : dvalue -> Prop :=
+    | d_addr: forall addr,
+        serialize_defined (DVALUE_Addr addr)
+    | d_i1: forall i1,
+        serialize_defined (DVALUE_I1 i1)
+    | d_i8: forall i1,
+        serialize_defined (DVALUE_I8 i1)
+    | d_i32: forall i32,
+        serialize_defined (DVALUE_I32 i32)
+    | d_i64: forall i64,
+        serialize_defined (DVALUE_I64 i64)
+    | d_struct_empty:
+        serialize_defined (DVALUE_Struct [])
+    | d_struct_nonempty: forall dval fields_list,
+        serialize_defined dval ->
+        serialize_defined (DVALUE_Struct fields_list) ->
+        serialize_defined (DVALUE_Struct (dval :: fields_list))
+    | d_array_empty:
+        serialize_defined (DVALUE_Array [])
+    | d_array_nonempty: forall dval fields_list,
+        serialize_defined dval ->
+        serialize_defined (DVALUE_Array fields_list) ->
+        serialize_defined (DVALUE_Array (dval :: fields_list)).
 
-  (* Todo - complete proofs, and think about moving to MemoryProp module. *)
-  (* The relation defining serializable dvalues. *)
-  Inductive serialize_defined : dvalue -> Prop :=
-  | d_addr: forall addr,
-      serialize_defined (DVALUE_Addr addr)
-  | d_i1: forall i1,
-      serialize_defined (DVALUE_I1 i1)
-  | d_i8: forall i1,
-      serialize_defined (DVALUE_I8 i1)
-  | d_i32: forall i32,
-      serialize_defined (DVALUE_I32 i32)
-  | d_i64: forall i64,
-      serialize_defined (DVALUE_I64 i64)
-  | d_struct_empty:
-      serialize_defined (DVALUE_Struct [])
-  | d_struct_nonempty: forall dval fields_list,
-      serialize_defined dval ->
-      serialize_defined (DVALUE_Struct fields_list) ->
-      serialize_defined (DVALUE_Struct (dval :: fields_list))
-  | d_array_empty:
-      serialize_defined (DVALUE_Array [])
-  | d_array_nonempty: forall dval fields_list,
-      serialize_defined dval ->
-      serialize_defined (DVALUE_Array fields_list) ->
-      serialize_defined (DVALUE_Array (dval :: fields_list)).
+    (* Lemma assumes all integers encoded with 8 bytes. *)
 
-  (* Lemma assumes all integers encoded with 8 bytes. *)
-
-  Inductive sbyte_list_wf : list SByte -> Prop :=
-  | wf_nil : sbyte_list_wf []
-  | wf_cons : forall b l, sbyte_list_wf l -> sbyte_list_wf (Byte b :: l)
-  .
+    Inductive sbyte_list_wf : list SByte -> Prop :=
+    | wf_nil : sbyte_list_wf []
+    | wf_cons : forall b l, sbyte_list_wf l -> sbyte_list_wf (Byte b :: l)
+    .
 
   (*
 Lemma sbyte_list_to_Z_inverse:
@@ -345,7 +416,6 @@ Proof.
   intros i1.
   destruct i1. simpl.
 Admitted. *)
-
 
   (*
 Lemma serialize_inverses : forall dval,
@@ -375,213 +445,296 @@ Proof.
 Admitted.
    *)
 
-  (* Construct block indexed from 0 to n. *)
-  Fixpoint init_block_h (n:nat) (m:mem_block) : mem_block :=
-    match n with
-    | O => add 0 SUndef m
-    | S n' => add (Z.of_nat n) SUndef (init_block_h n' m)
-    end.
+  End Serialization.
 
-  (* Initializes a block of n 0-bytes. *)
-  Definition init_block (n:Z) : mem_block :=
-    match n with
-    | 0 => empty
-    | Z.pos n' => init_block_h (BinPosDef.Pos.to_nat (n' - 1)) empty
-    | Z.neg _ => empty (* invalid argument *)
-    end.
+  Section GEP.
 
-  (* Makes a block appropriately sized for the given type. *)
-  Definition make_empty_mem_block (ty:dtyp) : mem_block :=
-    init_block (sizeof_dtyp ty).
-
-  Definition make_empty_block (ty:dtyp) : logical_block :=
-    let block := make_empty_mem_block ty in
-    LBlock (sizeof_dtyp ty) block None.
-
-  Fixpoint handle_gep_h (t:dtyp) (off:Z) (vs:list dvalue): err Z :=
-    match vs with
-    | v :: vs' =>
-      match v with
-      | DVALUE_I32 i =>
-        let k := unsigned i in
-        let n := BinIntDef.Z.to_nat k in
-        match t with
-        | DTYPE_Vector _ ta
-        | DTYPE_Array _ ta =>
-          handle_gep_h ta (off + k * (sizeof_dtyp ta)) vs'
-        | DTYPE_Struct ts
-        | DTYPE_Packed_struct ts => (* Handle these differently in future *)
-          let offset := fold_left (fun acc t => acc + sizeof_dtyp t)
-                                  (firstn n ts) 0 in
-          match nth_error ts n with
-          | None => failwith "overflow"
-          | Some t' =>
-            handle_gep_h t' (off + offset) vs'
+    (** ** Get Element Pointer
+      Retrieve the address of a subelement of an indexable (i.e. aggregate) [dtyp] [t] (i.e. vector, array, struct, packed struct).
+      The [off]set parameter contains the current entry address of the aggregate structure being analyzed, while the list
+      of [dvalue] [vs] describes the indexes of interest used to access the subelement.
+      The interpretation of these values slightly depends on the type considered.
+      But essentially, for instance in a vector or an array, the head value should be an [i32] describing the index of interest.
+      The offset is therefore incremented by this index times the size of the type of elements stored. Finally, a recursive call
+      at this new offset allows for deeper unbundling of a nested structure.
+     *)
+    Fixpoint handle_gep_h (t:dtyp) (off:Z) (vs:list dvalue): err Z :=
+      match vs with
+      | v :: vs' =>
+        match v with
+        | DVALUE_I32 i =>
+          let k := unsigned i in
+          let n := BinIntDef.Z.to_nat k in
+          match t with
+          | DTYPE_Vector _ ta
+          | DTYPE_Array _ ta =>
+            handle_gep_h ta (off + k * (sizeof_dtyp ta)) vs'
+          | DTYPE_Struct ts
+          | DTYPE_Packed_struct ts => (* Handle these differently in future *)
+            let offset := fold_left (fun acc t => acc + sizeof_dtyp t)
+                                    (firstn n ts) 0 in
+            match nth_error ts n with
+            | None => failwith "overflow"
+            | Some t' =>
+              handle_gep_h t' (off + offset) vs'
+            end
+          | _ => failwith ("non-i32-indexable type")
           end
-        | _ => failwith ("non-i32-indexable type")
+        | DVALUE_I8 i =>
+          let k := unsigned i in
+          let n := BinIntDef.Z.to_nat k in
+          match t with
+          | DTYPE_Vector _ ta
+          | DTYPE_Array _ ta =>
+            handle_gep_h ta (off + k * (sizeof_dtyp ta)) vs'
+          | _ => failwith ("non-i8-indexable type")
+          end
+        | DVALUE_I64 i =>
+          let k := unsigned i in
+          let n := BinIntDef.Z.to_nat k in
+          match t with
+          | DTYPE_Vector _ ta
+          | DTYPE_Array _ ta =>
+            handle_gep_h ta (off + k * (sizeof_dtyp ta)) vs'
+          | _ => failwith ("non-i64-indexable type")
+          end
+        | _ => failwith "non-I32 index"
         end
-      | DVALUE_I8 i =>
-        let k := unsigned i in
-        let n := BinIntDef.Z.to_nat k in
-        match t with
-        | DTYPE_Vector _ ta | DTYPE_Array _ ta =>
-                              handle_gep_h ta (off + k * (sizeof_dtyp ta)) vs'
-        | _ => failwith ("non-i8-indexable type")
+      | [] => ret off
+      end.
+
+    (* At the toplevel, GEP takes a [dvalue] as an argument that must contain a pointer, but no other pointer can be recursively followed.
+     The pointer set the block into which we look, and the initial offset. The first index value add to the initial offset passed to
+     [handle_gep_h] for the actual access to structured data.
+     *)
+    Definition handle_gep (t:dtyp) (dv:dvalue) (vs:list dvalue) : err dvalue :=
+      match vs with
+      | DVALUE_I32 i :: vs' => (* TODO: Handle non i32 / i64 indices *)
+        match dv with
+        | DVALUE_Addr (b, o) =>
+          off <- handle_gep_h t (o + (sizeof_dtyp t) * (unsigned i)) vs' ;;
+          ret (DVALUE_Addr (b, off))
+        | _ => failwith "non-address"
         end
-      | DVALUE_I64 i =>
-        let k := unsigned i in
-        let n := BinIntDef.Z.to_nat k in
-        match t with
-        | DTYPE_Vector _ ta
-        | DTYPE_Array _ ta =>
-          handle_gep_h ta (off + k * (sizeof_dtyp ta)) vs'
-        | _ => failwith ("non-i64-indexable type")
+      | DVALUE_I64 i :: vs' =>
+        match dv with
+        | DVALUE_Addr (b, o) =>
+          off <- handle_gep_h t (o + (sizeof_dtyp t) * (unsigned i)) vs' ;;
+          ret (DVALUE_Addr (b, off))
+        | _ => failwith "non-address"
         end
       | _ => failwith "non-I32 index"
-      end
-    | [] => ret off
-    end.
+      end.
 
-  Definition handle_gep (t:dtyp) (dv:dvalue) (vs:list dvalue) : err dvalue :=
-    match vs with
-    | DVALUE_I32 i :: vs' => (* TODO: Handle non i32 / i64 indices *)
-      match dv with
-      | DVALUE_Addr (b, o) =>
-        off <- handle_gep_h t (o + (sizeof_dtyp t) * (unsigned i)) vs' ;;
-        ret (DVALUE_Addr (b, off))
-      | _ => failwith "non-address"
-      end
-    | DVALUE_I64 i :: vs' =>
-      match dv with
-      | DVALUE_Addr (b, o) =>
-        off <- handle_gep_h t (o + (sizeof_dtyp t) * (unsigned i)) vs' ;;
-        ret (DVALUE_Addr (b, off))
-      | _ => failwith "non-address"
-      end
-    | _ => failwith "non-I32 index"
-    end.
+  End GEP.
+
+  Section Logical_Operations.
+
+    Definition logical_empty : logical_memory := empty.
+
+    (* Returns a fresh key for use in memory map *)
+    Definition logical_next_key (m : logical_memory) : Z
+      := let keys := map fst (IM.elements m) in
+         1 + maximumBy Z.leb (-1) keys.
+
+    (** ** Initialization of blocks
+      Constructs an initial [mem_block] of undefined [SByte]s, indexed from 0 to n.
+     *)
+    Fixpoint init_block_undef (n:nat) (m:mem_block) : mem_block :=
+      match n with
+      | O => add 0 SUndef m
+      | S n' => add (Z.of_nat n) SUndef (init_block_undef n' m)
+      end.
+
+    (* Constructs an initial [mem_block] containing [n] undefined [SByte]s, indexed from [0] to [n - 1].
+     If [n] is negative, it is treated as [0].
+     *)
+    Definition init_block (n:Z) : mem_block :=
+      match n with
+      | 0 => empty
+      | Z.pos n' => init_block_undef (BinPosDef.Pos.to_nat (n' - 1)) empty
+      | Z.neg _ => empty (* invalid argument *)
+      end.
+
+    (* Constructs an initial [mem_block] appropriately sized for a given type [ty]. *)
+    Definition make_empty_mem_block (ty:dtyp) : mem_block :=
+      init_block (sizeof_dtyp ty).
+
+    (* Constructs an initial [logical_block] appropriately sized for a given type [ty]. *)
+    Definition make_empty_block (ty:dtyp) : logical_block :=
+      let block := make_empty_mem_block ty in
+      LBlock (sizeof_dtyp ty) block None.
+
+  End Logical_Operations.
+  
+  Section Concrete_Operations.
+
+    Definition concrete_empty : concrete_memory := empty.
+
+    Definition concrete_next_key (m : concrete_memory) : Z :=
+      let keys         := List.map fst (IM.elements m) in
+      let max          := max_default keys 0 in
+      let offset       := 1 in (* TODO: This should be "random" *)
+      match lookup max m with
+      | None => offset
+      | Some (CBlock sz _) => max + sz + offset
+      end.
+
+  End Concrete_Operations.
+
+  Section Memory_Operations.
+
+      (** ** Smart lookups *)
+      Definition lookup_concrete (b : Z) (m : memory) : option concrete_block :=
+        let concrete_map := fst m in
+        lookup b concrete_map.
+
+      Definition lookup_logical (b : Z) (m : memory) : option logical_block :=
+        let logical_map := snd m in
+        lookup b logical_map.
+
+      (* Get the next key in the logical map *)
+      Definition next_key_logical (m : memory) : Z :=
+        logical_next_key (snd m).
+      
+      (* Get the next key in the concrete map *)
+      Definition next_key_concrete (m : memory) : Z :=
+        concrete_next_key (fst m).
+
+      (** ** Extending the memory  *)
+      Definition add_concrete (id : Z) (b : concrete_block) (m : memory) : memory :=
+        match m with
+        | (cm, lm) =>
+          (add id b cm, lm)
+        end.
+
+      Definition add_logical (id : Z) (b : logical_block) (m : memory) : memory :=
+        match m with
+        | (cm, lm) =>
+          (cm, add id b lm)
+        end.
+      
+      (** ** Concretization of blocks
+          Look-ups a concrete block in memory. The logical memory acts first as a potential layer of indirection:
+          - if no logical block is found, the input is directly returned.
+          - if a logical block is found, and that a concrete block is associated, the address of this concrete block
+          is returned, paired with the input memory.
+          - if a logical block is found, but that no concrete block is (yet) associated to it, then the associated
+          concrete block is allocated, and the association is added to the logical block.
+       *)
+      Definition concretize_block (b:Z) (m:memory) : Z * memory :=
+        match lookup_logical b m with
+        | None => (b, m) (* TODO: Not sure this makes sense??? *)
+        | Some (LBlock sz bytes (Some cid)) => (cid, m)
+        | Some (LBlock sz bytes None) =>
+          (* Allocates a concrete block for this one *)
+          let id        := next_key_concrete m in
+          let new_block := CBlock sz b in
+          let m'        := add_concrete id new_block m in
+          let m''       := add_logical  b (LBlock sz bytes (Some id)) m' in
+          (id, m'')
+        end.
+
+      (** ** Abstraction of blocks
+          Retrieve a logical description of a block as address and offset from its concrete address.
+          The non-trivial part consists in extracting from the [concrete_memory] the concrete address
+          and block corresponding to a logical one.
+       *)
+      Definition get_real_cid (cid : Z) (m : memory) : option (Z * concrete_block)
+        := IM.fold (fun k '(CBlock sz bid) a => if (k <=? cid) && (cid <? k + sz)
+                                             then Some (k, CBlock sz bid)
+                                             else a) (fst m) None.
+
+      Definition concrete_address_to_logical (cid : Z) (m : memory) : option (Z * Z)
+        := match m with
+           | (cm, lm) =>
+             '(rid, CBlock sz bid) <- get_real_cid cid m ;;
+             ret (bid, cid-rid)
+           end.
+
+      (* LLVM 5.0 memcpy
+         According to the documentation: http://releases.llvm.org/5.0.0/docs/LangRef.html#llvm-memcpy-intrinsic
+         this operation can never fail?  It doesn't return any status code...
+       *)
+      
+      (* TODO probably doesn't handle sizes correctly... *)
+      (** ** MemCopy
+          Implementation of the [memcpy] intrinsics.
+       *)
+      Definition handle_memcpy (args : list dvalue) (m:memory) : err memory :=
+        match args with
+        | DVALUE_Addr (dst_b, dst_o) ::
+                      DVALUE_Addr (src_b, src_o) ::
+                      DVALUE_I32 len ::
+                      DVALUE_I32 align :: (* alignment ignored *)
+                      DVALUE_I1 volatile :: [] (* volatile ignored *)  =>
+
+          src_block <- trywith "memcpy src block not found" (lookup_logical src_b m) ;;
+          dst_block <- trywith "memcpy dst block not found" (lookup_logical dst_b m) ;;
+
+          let src_bytes
+              := match src_block with
+                 | LBlock size bytes concrete_id => bytes
+                 end in
+          let '(dst_sz, dst_bytes, dst_cid)
+              := match dst_block with
+                 | LBlock size bytes concrete_id => (size, bytes, concrete_id)
+                 end in
+          let sdata := lookup_all_index src_o (unsigned len) src_bytes SUndef in
+          let dst_bytes' := add_all_index sdata dst_o dst_bytes in
+          let dst_block' := LBlock dst_sz dst_bytes' dst_cid in
+          let m' := add_logical dst_b dst_block' m in
+          (ret m' : err memory)
+        | _ => failwith "memcpy got incorrect arguments"
+        end.
+
+  End Memory_Operations.
+
+  Section Frame_Stack_Operations.
+
+    (* The initial frame stack is not an empty stack, but a singleton stack containing an empty frame *)
+    Definition frame_empty : frame_stack := [[]].
+
+    (** ** Free
+        [free_frame f m] deallocates the frame [f] from the memory [m].
+        This acts on both representations of the memory:
+        - on the logical memory, it simply removes all keys indicated by the frame;
+        - on the concrete side, for each element of the frame, we lookup in the logical memory
+        if it is bounded to a logical block, and if so if this logical block contains an associated
+        concrete block. If so, we delete this association from the concrete memory.
+     *)
+    Definition free_concrete_of_logical
+               (b : Z)
+               (lm : logical_memory)
+               (cm : concrete_memory) : concrete_memory
+      := match lookup b lm with
+         | None => cm
+         | Some (LBlock _ _ None) => cm
+         | Some (LBlock _ _ (Some cid)) => delete cid cm
+         end.
+
+    Definition free_frame (f : mem_frame) (m : memory) : memory := 
+      let '(cm, lm) := m in
+      let cm' := fold_left (fun m key => free_concrete_of_logical key lm m) f cm in
+      (cm', fold_left (fun m key => delete key m) f lm).
+    
+  End Frame_Stack_Operations.
+
+  Section Memory_Stack_Operations.
+
+    (** ** The empty memory
+        Both the concrete and logical views of the memory are empty maps, i.e. nothing is allocated.
+        It is a matter of convention, by we consider the empty memory to contain a single empty frame
+        in its stack, rather than an empty stack.
+     *)
+    Definition empty_memory_stack : memory_stack := ((concrete_empty, logical_empty), frame_empty).
+
+  End Memory_Stack_Operations.
 
 
-  Definition lookup_concrete (b : Z) (m : memory) : option concrete_block :=
-    let concrete_map := fst m in
-    lookup b concrete_map.
-
-  Definition lookup_logical (b : Z) (m : memory) : option logical_block :=
-    let logical_map := snd m in
-    lookup b logical_map.
-
-  (* Get next key in logical map *)
-  Definition next_logical_key (m : memory) : Z :=
-    next_key (snd m).
-
-
-  (* Get next key in concrete map *)
-  Definition next_concrete_key (m : memory) : Z :=
-    let concrete_map := fst m in
-    let keys         := List.map fst (IM.elements concrete_map) in
-    let max          := max_default keys 0 in
-    let offset       := 1 in (* TODO: This should be "random" *)
-    match lookup_concrete max m with
-    | None => offset
-    | Some (CBlock sz _) => max + sz + offset
-    end.
-
-  Definition add_concrete (id : Z) (b : concrete_block) (m : memory) : memory :=
-    match m with
-    | (cm, lm) =>
-      (add id b cm, lm)
-    end.
-
-  Definition add_logical (id : Z) (b : logical_block) (m : memory) : memory :=
-    match m with
-    | (cm, lm) =>
-      (cm, add id b lm)
-    end.
-
-  Definition concretize_block (b:Z) (m:memory) : Z * memory :=
-    match lookup_logical b m with
-    | None => (b, m) (* TODO: Not sure this makes sense ??? *)
-    | Some (LBlock sz bytes (Some cid)) => (cid, m)
-    | Some (LBlock sz bytes None) =>
-      (* Allocate a concrete block for this one *)
-      let id        := next_concrete_key m in
-      let new_block := CBlock sz b in
-      let m'        := add_concrete id new_block m in
-      let m''       := add_logical  b (LBlock sz bytes (Some id)) m' in
-      (id, m'')
-    end.
-
-  (* LLVM 5.0 memcpy
-   According to the documentation: http://releases.llvm.org/5.0.0/docs/LangRef.html#llvm-memcpy-intrinsic
-   this operation can never fail?  It doesn't return any status code...
+  (** ** Memory Handler
+      Implementation of the memory model per se as a memory handler to the [MemoryE] interface.
    *)
-
-  (* TODO probably doesn't handle sizes correctly... *)
-  Definition handle_memcpy (args : List.list dvalue) (m:memory) : err memory :=
-    match args with
-    | DVALUE_Addr (dst_b, dst_o) ::
-      DVALUE_Addr (src_b, src_o) ::
-      DVALUE_I32 len ::
-      DVALUE_I32 align :: (* alignment ignored *)
-      DVALUE_I1 volatile :: [] (* volatile ignored *)  =>
-
-      src_block <- trywith "memcpy src block not found" (lookup_logical src_b m) ;;
-      dst_block <- trywith "memcpy dst block not found" (lookup_logical dst_b m) ;;
-
-      let src_bytes
-          := match src_block with
-             | LBlock size bytes concrete_id => bytes
-             end in
-      let '(dst_sz, dst_bytes, dst_cid)
-          := match dst_block with
-             | LBlock size bytes concrete_id => (size, bytes, concrete_id)
-             end in
-      let sdata := lookup_all_index src_o (unsigned len) src_bytes SUndef in
-      let dst_bytes' := add_all_index sdata dst_o dst_bytes in
-      let dst_block' := LBlock dst_sz dst_bytes' dst_cid in
-      let m' := add_logical dst_b dst_block' m in
-      (ret m' : err memory)
-    | _ => failwith "memcpy got incorrect arguments"
-    end.
-
-  (* TODO:
-   - we can use the handler combinators to make these more modular
-
-   - these operations are too defined: load and store should fail if the
-     address isn't in range
-   *)
-
-  Definition free_concrete_of_logical
-             (b : Z)
-             (lm : logical_memory)
-             (cm : concrete_memory) : concrete_memory
-    := match lookup b lm with
-       | None => cm
-       | Some (LBlock _ _ None) => cm
-       | Some (LBlock _ _ (Some cid)) => delete cid cm
-       end.
-
-  Definition free_frame (f : mem_frame) (m : memory) : memory
-    := match m with
-       | (cm, lm) =>
-         let cm' := fold_left (fun m key => free_concrete_of_logical key lm m) f cm in
-         (cm', fold_left (fun m key => delete key m) f lm)
-       end.
-
-  (* Get the cid stored in the memory map *)
-  Definition get_real_cid (cid : Z) (m : memory) : option (Z * concrete_block)
-    := IM.fold (fun k '(CBlock sz bid) a => if (k <=? cid) && (cid <? k + sz)
-                                         then Some (k, CBlock sz bid)
-                                         else a) (fst m) None.
-
-  (* Convert a concrete address to a block and offset *)
-  Definition concrete_address_to_logical (cid : Z) (m : memory) : option (Z * Z)
-    := match m with
-       | (cm, lm) =>
-         '(rid, CBlock sz bid) <- get_real_cid cid m ;;
-          ret (bid, cid-rid)
-       end.
-
   Definition handle_memory {E} `{FailureE -< E} `{UBE -< E}: MemoryE ~> stateT memory_stack (itree E) :=
     fun _ e '(m, s) =>
       match e with
@@ -597,7 +750,7 @@ Admitted.
 
       | Alloca t =>
         let new_block := make_empty_block t in
-        let key := next_logical_key m in
+        let key := next_key_logical m in
         let new_mem := add_logical key new_block m in
 
         match s with
